## 1

(1)

$$y_{n+1}=y_n+0.2*(x_n^2-y_n^2)$$

(2)

$$y_{n+1}=y_n+0.1*\left(\left(\frac{y_n}{x_n}\right)^2-\frac{y_n}{x_n}\right)$$

---

## 4

$y'(x)=f(x,y)$

等效格式

$$y_{n+1}=ay_n+by_{n-1}+h(c*y'(x_n)+d*y'(x_{n-1}))$$

令 $n=0,h=1$

即

$$y_{1}=ay_0+by_{-1}+c*y'(x_0)+d*y'(x_{-1})$$

考察对应的近似关系式

$$y(1)=ay(0)+by(-1)+c*y'(0)+d*y'(-1)$$

$y=1,y'=0$ 时

$$\tag{1}1=a+b$$

$y=x,y'=1$ 时

$$\tag{2}1=a*0+b*(-1)+c*1+d*1$$

$y=x^2,y'=2x$ 时

$$\tag{3}1=b-2d$$

$y=x^3,y'=3x^2$ 时

$$\tag{4}1=a*0+b*(-1)+c*0+d*3$$

由 (1)(2)(3)(4) 解得

$a = -4, b = 5, c = 4, d = 2$

检验 $y=x^4,y'=4x^3$

$1\ne 5+(-4)*2$

所以两步格式为

$$y_{n+1}=-4y_n+5y_{n-1}+1(4*f(x_n,y_n)+2*f(x_{n-1},y_{n-1}))$$

3 阶精度

---

## 5

$y'(x)=f(x,y)$

$y'(x)=-y(x)$

梯形公式：$y_{n+1}=y_n+\dfrac{h}{2}[y'(x_n)+y'(x_{n+1})]$

即

$$y_{n+1}=y_n+\dfrac{h}{2}[-y(x_n)-y(x_{n+1})]=y_n+\dfrac{h}{2}[-y_n-y_{n+1}]$$

$$
y_{n+1}=\left(\frac{2-h}{2+h}\right)y_n,y(0)=1
$$

解递推方程得 $y_n=\left(\dfrac{2-h}{2+h}\right)^n$

$$
\begin{aligned}
&\lim_{h\to 0}\left(\dfrac{2-h}{2+h}\right)^n\\
=&\lim_{h\to 0}\left(1+\dfrac{-2h}{2+h}\right)^n\\
=&\lim_{h\to 0}\left[\left(1+\dfrac{-2h}{2+h}\right)^{\dfrac{2+h}{-2h}}\right]^{\dfrac{-2hn}{2+h}}\\
=&\lim_{h\to 0}e^{\dfrac{-2x_n}{2+h}}\\
=&\lim_{h\to 0}e^{\dfrac{-2x_n}{2}}\\
=&e^{-x_n}\\
\end{aligned}
$$

所以 $h\to 0$ 时，收敛到 $y=e^{-x}$

---

## 8

$n=0,h=1$

得到近似关系式为

$$y(1)=(1-b)y(0)+by(-1)+1/4*((b+3)y'(1)+(3b+1)y'(-1))$$

$y=1,y'=0$ 时

$$\tag{1}1=1-b+b$$

恒成立

$y=x,y'=1$ 时

$$\tag{2}1=-b+1/4*(b+3+3b+1)$$

恒成立

$y=x^2,y'=2x$ 时

$$\tag{3}1=b+1/4*(2(b+3))+(3b+1)(-2))$$

恒成立

$y=x^3,y'=3x^2$ 时

$$\tag{4}1=-b+1/4*(3(b+3)+(3b+1)*3)$$

解得 $b=-1$

所以 $b=-1$ 时 3 阶，$b\ne -1$ 时 2 阶