# 1

计算 1 式得

$$
\tag{1}x_1=3+\frac{1}{2}x_2
$$

代入 2 式得

$$
-x_1+3x_2-2x_3=1
$$

解得

$$
\tag{2}x_2= \frac{4}{5} (x_3+2)
$$

类推得

$$
\tag{3}x_3= \frac{1}{6} (5 x_4+8)
$$

$$
\tag{4}x_4=2
$$

回代解得

$$
\{x_1,x_2,x_3,x_4\}=\{5,4,3,2\}
$$

---

# 5

$$
\begin{bmatrix}
    {a} & {0} & {0}\\
    {b} & {c} & {0}\\
    {d} & {e} & {f}\\
\end{bmatrix}
\begin{bmatrix}
    {a} & {0} & {0}\\
    {b} & {c} & {0}\\
    {d} & {e} & {f}\\
\end{bmatrix}^T=\begin{bmatrix}
 a^2 & a b & a d \\
 a b & b^2+c^2 & b d+c e \\
 a d & b d+c e & d^2+e^2+f^2 \\
\end{bmatrix}=\begin{bmatrix}
    {3} & {2} & {3}\\
    {2} & {2} & {0}\\
    {3} & {0} & {12}\\
\end{bmatrix}
$$

$$
a= \sqrt{3},b= \frac{2}{\sqrt{3}},c= \sqrt{\frac{2}{3}},d= \sqrt{3},e= -\sqrt{6},f= \sqrt{3}
$$

---

# 7

将矩阵 $L_1U$ 分解得

$$
\begin{bmatrix}
 1 & 0 & 0 & 0 \\
 \frac{7}{5} & 1 & 0 & 0 \\
 1 & 0 & 1 & 0 \\
 \frac{6}{5} & -2 & \frac{10}{3} & 1 \\
\end{bmatrix}
\begin{bmatrix}
 5 & 7 & 9 & 10 \\
 0 & \frac{1}{5} & -\frac{23}{5} & -7 \\
 0 & 0 & -3 & -5 \\
 0 & 0 & 0 & -\frac{1}{3} \\
\end{bmatrix}
$$

从而解得

$x_1=20,x_2=-12,x_3=-5,x_4=3$

---